finish sem_typ_top_abs

systemt/extensional/per.v
@@ -1,1 +1,65 @@
+Require Import nbe.systemt.extensional.syntax.
 Require Import nbe.systemt.extensional.semantic.
+
+Definition SemTyp := D -> D -> Prop.
+
+Notation "d ∈! T" := (T d d) 
+ (at level 55, no associativity).
+
+Definition SemTypTop (d d' : Dnf) : Prop :=
+  forall n, exists w, Rⁿᶠ ⦇ n ⦈ d ↘ w /\ Rⁿᶠ ⦇ n ⦈ d' ↘ w.
+
+Definition SemTypBot (e e' : Dne) : Prop :=
+  forall n, exists u, Rⁿᵉ ⦇ n ⦈ e ↘ u /\ Rⁿᵉ ⦇ n ⦈ e' ↘ u.
+
+Notation " e ≈ e' ∈ ⊥" := (SemTypBot e e')
+  (at level 55, no associativity).
+
+Notation " d ≈ d' ∈ ⊤" := (SemTypTop d d')
+  (at level 55, no associativity).
+
+Hint Constructors RNfRel RNeRel : core.
+
+Lemma sem_typ_bot_var : forall i,
+  (dne_l i) ≈ (dne_l i) ∈ ⊥.
+Proof.
+  intros. unfold SemTypBot. intros.
+  exists (ne_v (n - i - 1)). split; eauto.
+Qed.
+
+Lemma sem_typ_bot_app : forall e e' d d',
+  e ≈ e' ∈ ⊥ ->
+  d ≈ d' ∈ ⊤ ->
+  (dne_app e d) ≈ (dne_app e' d') ∈ ⊥.
+Proof.
+  intros. unfold SemTypBot in *. unfold SemTypTop in *. intros.
+  specialize (H n).
+  specialize (H0 n).
+  destruct H as [u [Hrnee Hrnee']].
+  destruct H0 as [w [Hrnfd Hrnfd']].
+  exists (ne_app u w). intuition.
+Qed.
+
+Lemma sem_typ_top_ne : forall e e',
+  e ≈ e' ∈ ⊥ ->
+  dnf_reif ℕ (d_refl ℕ e) ≈ dnf_reif ℕ (d_refl ℕ e') ∈ ⊤.
+Proof.
+  intros. unfold SemTypTop. unfold SemTypBot in *. intros.
+  specialize (H n).
+  destruct H as [u [Hrnee Hrnee']].
+  exists (nf_ne u). intuition.
+Qed.
+
+Lemma sem_typ_top_abs : forall f f' S T,
+  (forall e e', e ≈ e' ∈ ⊥ -> 
+    exists b b', f ∙ (d_refl S e) ↘ b /\ f' ∙ (d_refl S e') ↘ b' /\ 
+      (dnf_reif T b) ≈ (dnf_reif T b') ∈ ⊤) ->
+  (dnf_reif (S → T) f) ≈ (dnf_reif (S → T) f') ∈ ⊤.
+Proof.
+  intros. unfold SemTypTop. intros.
+  assert (dne_l n ≈ dne_l n ∈ ⊥) by (unfold SemTypBot; intros; eauto).
+  apply H in H0.
+  destruct H0 as [b [b']]. intuition.
+  unfold SemTypTop in H3. specialize (H3 (1 + n)). destruct H3 as [w].
+  exists (nf_abs w); intuition; eauto.
+Qed.
